example/TestSdiv.thy
@@ -1,0 +1,68 @@
+theory TestSdiv
+
+imports Main "../ContractSem"
+
+begin
+
+declare eval_annotation_def [simp]
+
+definition this_address :: address
+where "this_address = undefined"
+
+abbreviation test_sdiv_code :: "inst list"
+where
+"test_sdiv_code ==
+   Stack (PUSH_N [255])
+ # Stack (PUSH_N [2])
+ # Arith EXP
+ # Dup 1
+ # Annotation (\<lambda> aenv. length (aenv_stack aenv) = 2)
+ # Stack (PUSH_N [0])
+ # Bits inst_NOT
+ # Swap 1
+ # Annotation (\<lambda> aenv. length (aenv_stack aenv) = 3)
+ # Sarith SDIV
+ # Annotation (\<lambda> aenv. length (aenv_stack aenv) = 2)
+ # Annotation (\<lambda> aenv. (aenv_stack aenv ! 0) = (aenv_stack aenv ! 1))
+ # Misc STOP
+ # []"
+
+
+ 
+abbreviation test_sdiv_account_state :: "account_state"
+where
+"test_sdiv_account_state ==
+   \<lparr> account_address = this_address
+   , account_storage = \<lambda> _. 0
+   , account_code = test_sdiv_code
+   , account_balance = 0
+   , account_ongoing_calls = []
+   \<rparr>"
+
+abbreviation test_sdiv_spec :: "response_to_world"
+where
+" test_sdiv_spec ==
+  \<lparr> when_called = \<lambda> _. (ContractReturn [],
+                        \<lambda> a. True)
+  , when_returned = \<lambda> _. (ContractFail,
+                           \<lambda> a. True)
+  , when_failed = (ContractFail,
+                     \<lambda> a. True)
+  \<rparr>
+"
+
+value "32 div sint (max_word :: uint)"
+
+lemma test_sdiv_correct:
+"
+  account_state_responds_to_world
+  (\<lambda> a. a = test_sdiv_account_state)
+  test_sdiv_spec
+"
+apply(rule AccountStep; auto)
+apply(case_tac steps; auto)
+apply(simp add:max_word_def)
+apply(simp add:max_word_def)
+done
+
+end
